theories/c_interop/rules.v
@@ -356,7 +356,7 @@ Qed.
 (*   registerroot_proto ⊑ Ψ → *)
 (*   (⊢ GC θ -∗ *)
 (*      (▷ ∀ (l : loc), GC θ ∗ l ↦roots Lint 0 -∗ *)
-(*      WP (subst_all {[n := Val #C l]} ∅ e2) at ⟨ p, Ψ ⟩ {{Φ}}) -∗ *)
+(*      WP (subst_all {[n := #C l]} e2) at ⟨ p, Ψ ⟩ {{Φ}}) -∗ *)
 (*      WP (CAMLlocal: n in e2)%CE at ⟨ p, Ψ ⟩ {{Φ}}%CE)%I. *)
 (* Proof. *)
 (*   iIntros (????) "HGC Cont". unfold CAMLlocal. *)
