theories/c_lang/notation.v
@@ -43,7 +43,9 @@ Notation "e1 = e2" := (BinOp EqOp e1%CE e2%CE) : c_expr_scope.
 Notation "e1 ≠ e2" := (UnOp NotOp (BinOp EqOp e1%CE e2%CE)) : c_expr_scope.
 (* The unicode ← is already part of the notation "_ ← _; _" for bind. *)
 Notation "e1 <- e2" := (Store e1%CE e2%CE) (at level 80, e2 at level 78) : c_expr_scope.
-
+Notation "e <- '[' v1 , .. , vn ']'" :=
+  (store_array e%CE (@cons (option val) v1%CE .. (@cons (option val) vn%CE nil) ..))
+  (at level 80).
 
 Notation "'if:' e1 'then' e2 'else' e3" := (If e1%CE e2%CE e3%CE)
   (at level 200, e1, e2, e3 at level 200) : c_expr_scope.
@@ -51,7 +53,8 @@ Notation "'if:' e1 'then' e2 'else' e3" := (If e1%CE e2%CE e3%CE)
 Notation "'while:' e1 'do' e2" := (While e1%CE e2%CE)
   (at level 200, e1, e2 at level 200) : c_expr_scope.
 
-Notation "'call:' ff 'with' '(' e1 , .. , en ')'" := (FunCall ff%CE (@cons expr e1%CE .. (@cons expr en%CE nil) ..))
+Notation "'call:' ff 'with' '(' e1 , .. , en ')'" :=
+  (FunCall ff%CE (@cons expr e1%CE .. (@cons expr en%CE nil) ..))
   (at level 70) : c_expr_scope.
 
 Notation "'call:' ff 'with' '(' ')'" := (FunCall ff%CE nil)
