theories/examples/is_eq.v
@@ -41,7 +41,7 @@ Definition is_eq_code (x_arg y_arg : expr) : C_lang.expr :=
    call: &"int2val" with ("res").
 
 Lemma is_eq_code_subst (wx wy : val) :
-  C_lang.subst_all (<["x_arg":=Val wx]> (<["y_arg":=Val wy]> ∅)) ∅ (is_eq_code "x_arg" "y_arg")
+C_lang.subst_all (<["x_arg":=wx]> (<["y_arg":=wy]> ∅)) (is_eq_code "x_arg" "y_arg")
   = (is_eq_code wx wy).
 Proof. done. Qed.
 
@@ -96,7 +96,7 @@ Section C_specs.
       { by iApply "Cont". } done.
     }
     iLöb as "IH" forall (τ x lvx wx y lvy wy Φ'' Hτ H1 H2).
-    wp_call_direct.
+    wp_allocframe fp "_".
     destruct τ => //=; iEval (unfold is_eq_code).
     - (* TUnit *)
       iDestruct "Hτx" as %->.
