theories/examples/swap_pair.v
@@ -55,8 +55,7 @@ Proof.
   destruct ws as [|w []]; try by (exfalso; apply Forall2_length in Hrepr; eauto with lia); [].
   apply Forall2_cons_1 in Hrepr as [Hrepr _].
   cbn. iDestruct "Hsim" as "[Hsim _]".
-  wp_call_direct.
-  wp_allocframe.
+  wp_allocframe fp "_".
 
   wp_pures.
   wp_alloc rr as "H"; first done.
